Verification for do 4.

code/Yazi.CRC32.fst
@@ -2,9 +2,11 @@ module Yazi.CRC32
 module B = LowStar.Buffer
 module BV = FStar.BitVector
 module Cast = FStar.Int.Cast
+module Math = FStar.Math.Lemmas
 module U32 = FStar.UInt32
 module UInt = FStar.UInt
 
+open FStar.Mul
 open FStar.Seq
 open LowStar.BufferOps
 open Spec.CRC32
@@ -45,43 +47,52 @@ let rec cast_zero_prefix (#n: nat) (v: UInt.uint_t n) (m: nat{m >= n}): Lemma
       assert(Seq.equal (UInt.to_vec #m v) ((Seq.create m false) @| (Seq.empty #bool)))
     end
 
-private unfold let u8_padding (b: U8.t) (n: nat{n > 32}): Tot (BV.bv_t n) =
-  (BV.zero_vec #24) @| (UInt.to_vec (U8.v b)) @| (BV.zero_vec #(n - 32))
+private unfold let u8_padding
+  (b: U8.t)
+  (n: nat{n > 0}):
+  Tot (BV.bv_t (32 + 8 * n)) =
+  (BV.zero_vec #24) @|
+  (UInt.to_vec (U8.v b)) @|
+  (BV.zero_vec #(8 * n))
 
-#set-options "--z3rlimit 120 --z3seed 1"
-let do1_logxor (#m: crc32_buf_len) (prev: BV.bv_t m) (crc: U32.t) (b: U8.t): Lemma
-  (requires crc32_matched #m prev crc false)
+#set-options "--z3rlimit 120 --z3seed 13 --fuel 0 --ifuel 0"
+let do1_logxor
+  (m: nat)
+  (data: Seq.seq U8.t{Seq.length data == m})
+  (crc: U32.t)
+  (b: U8.t): Lemma
+  (requires crc32_matched m data crc false)
   (ensures
     (m == 0 ==>
       UInt.to_vec (U32.v (U32.logxor crc (Cast.uint8_to_uint32 b))) ==
       (BV.ones_vec #32 +@ (zero_vec_l 24 (UInt.to_vec (U8.v b))))) /\
-    (m > 32 ==>
+    (m > 0 ==>
       UInt.to_vec (U32.v (U32.logxor crc (Cast.uint8_to_uint32 b))) ==
-      poly_mod (prev +@ (u8_padding b m)))) =
+      poly_mod ((crc32_data_to_bits m data) +@ (u8_padding b m)))) =
   let open U32 in
+  let buf = crc32_data_to_bits m data in
   let b32 = Cast.uint8_to_uint32 b in
-  let vb32: BV.bv_t 32 = UInt.to_vec (v b32) in
+  let vb32 = UInt.to_vec (v b32) in
   let vcrc = UInt.to_vec (v crc) in
+  let m' = 8 * m in
   cast_zero_prefix (U8.v b) 32;
-  if m > 32 then
+  if m > 0 then
     calc (==) {
       vcrc +@ vb32;
       =={}
-      (poly_mod prev) +@ vb32;
-      =={poly_mod_zero_suffix vb32 (m - 32)}
-      (poly_mod prev) +@ (poly_mod (zero_vec_r (m - 32) vb32));
-      =={
-        assert(Seq.equal (zero_vec_r (m - 32) vb32) (u8_padding b m))
-      }
-      (poly_mod prev) +@ (poly_mod (u8_padding b m));
-      =={poly_mod_add prev (u8_padding b m)}
-      poly_mod (prev +@ (u8_padding b m));
+      (poly_mod buf) +@ vb32;
+      =={poly_mod_zero_suffix vb32 m'}
+      (poly_mod buf) +@ (poly_mod (zero_vec_r m' vb32));
+      =={assert(Seq.equal (zero_vec_r m' vb32) (u8_padding b m))}
+      (poly_mod buf) +@ (poly_mod (u8_padding b m));
+      =={poly_mod_add buf (u8_padding b m)}
+      poly_mod (buf +@ (u8_padding b m));
     }
   else
-    ()
-
+    assert(Seq.equal (zero_vec_l 24 (UInt.to_vec (U8.v b))) vb32)
+  
 #set-options "--z3rlimit 200 --ifuel 128 --fuel 128 --z3seed 1"
-let logand_256 (r: U32.t): Lemma
+private let logand_256 (r: U32.t): Lemma
   (ensures forall (i: nat{i < 32}).
     (i < 32 - 8 ==> UInt.nth (U32.v (U32.logand r 0xFFul)) i == false) /\
     (i >= 32 - 8 ==> UInt.nth (U32.v (U32.logand r 0xFFul)) i == UInt.nth (U32.v r) i)) =
@@ -94,8 +105,8 @@ let logand_256 (r: U32.t): Lemma
     (i < 32 - 8 ==> UInt.nth (UInt.logand (v r) (v 0xFFul)) i == false) /\
     (i >= 32 - 8 ==> UInt.nth (UInt.logand (v r) (v 0xFFul)) i == UInt.nth (U32.v r) i))
 
-#set-options "--z3rlimit 200 --z3seed 1"
-let do1_shift_right_logxor (r: U32.t) (t: U32.t): Lemma
+#set-options "--z3seed 1 --fuel 0 --ifuel 0"
+private let do1_shift_right_logxor (r: U32.t) (t: U32.t): Lemma
   (requires poly_mod_correct 8 (U32.logand r 0xFFul) t)
   (ensures
      UInt.to_vec (U32.v (U32.logxor (U32.shift_right r 8ul) t)) ==
@@ -123,88 +134,245 @@ let do1_shift_right_logxor (r: U32.t) (t: U32.t): Lemma
     ((zero_vec_r 8 vr') +@ (zero_vec_l 8 vi))
     (zero_vec_l 8 (UInt.to_vec (U32.v r))))
 
+#set-options "--z3rlimit 200 --z3seed 1 --fuel 1 --ifuel 1"
 inline_for_extraction
 private let do1
-  (#m: Ghost.erased crc32_buf_len)
+  (m: Ghost.erased nat)
+  (data: Ghost.erased (Seq.seq U8.t){Seq.length data == Ghost.reveal m})
   (t8: Spec.table_buf)
-  (prev: Ghost.erased (BV.bv_t m))
   (crc: U32.t)
   (b: U8.t):
-  ST.Stack U32.t
-  (requires fun h -> table_correct 8 h t8 /\ crc32_matched #m prev crc false)
+  ST.Stack (U32.t & (Ghost.erased (Seq.seq U8.t)))
+  (requires fun h -> table_correct 8 h t8 /\ crc32_matched m data crc false)
   (ensures fun h0 res h1 ->
-    let curr = crc32_append_8bit #m prev b in
-    M.modifies M.loc_none h0 h1 /\
-    crc32_matched #(if Ghost.reveal m = 0 then 40 else m + 8) curr res false) =
+    let crc' = fst res in
+    let data' = Ghost.reveal (snd res) in
+    B.modifies B.loc_none h0 h1 /\
+    data' == data @| (Seq.create 1 b) /\
+    crc32_matched (m + 1) data' crc' false) =
   let b' = Cast.uint8_to_uint32 b in
   let open U32 in
-  let r = crc ^^ b' in 
+  let r = crc ^^ b' in
   UInt.logand_le (v r) (v 0xFFul);
   let tv = t8.(r &^ 0xFFul) in
   let r' = r >>^ 8ul in
   let p = r' ^^ tv in
+  let buf: Ghost.erased (BV.bv_t (if Ghost.reveal m = 0 then 0 else 32 + 8 * m)) =
+    Ghost.hide (crc32_data_to_bits m data)
+  in
+  do1_logxor m data crc b;
   do1_shift_right_logxor r tv;
-  do1_logxor prev crc b;
-  assert(UInt.to_vec (v p) == poly_mod (zero_vec_l 8 (UInt.to_vec (v r))));
-  if Ghost.reveal m = 0 then begin
-    assert(poly_mod (zero_vec_l 8 (UInt.to_vec (v r))) ==
-      poly_mod (zero_vec_l 8 (BV.ones_vec #32 +@ (zero_vec_l 24 (UInt.to_vec (U8.v b))))));
-    assert(Seq.equal
-      (zero_vec_l 8 (BV.ones_vec #32 +@ (zero_vec_l 24 (UInt.to_vec (U8.v b)))))
-      (crc32_append_8bit prev b))
-  end else begin
-    assert(poly_mod (zero_vec_l 8 (UInt.to_vec (v r))) ==
-      poly_mod (zero_vec_l 8 (poly_mod (prev +@ (u8_padding b m)))));
-    poly_mod_zero_prefix (prev +@ (u8_padding b m)) 8;
-    assert(Seq.equal
-      (zero_vec_l 8 (prev +@ (u8_padding b m)))
-      (crc32_append_8bit prev b))
-  end;
-  p
 
+  if Ghost.reveal m > 0 then begin
+    poly_mod_zero_prefix (buf +@ (u8_padding b m)) 8;
+    crc32_data_to_bits_append m 1 data (Seq.create 1 b)
+  end else
+    assert(Seq.equal (zero_vec_l 8 (UInt.to_vec (v r))) (crc32_append_8bit buf b));
+    
+  (p, Ghost.hide (data @| (Seq.create 1 b)))
+
+#set-options "--z3rlimit 200 --ifuel 0 --fuel 0 --z3seed 7"
 inline_for_extraction
 private let rec do1_remain
-  (t8: Spec.table_buf)
-  (l: U32.t)
-  (buf: B.buffer U8.t{B.length buf == U32.v l})
   (m: Ghost.erased nat)
-  (data: Ghost.erased (Seq.seq U8.t){Seq.length data == Ghost.reveal m})
-  (r: U32.t{U32.v r <= (U32.v l) % 4})
+  (prev: Ghost.erased (Seq.seq U8.t){Seq.length prev == Ghost.reveal m})
+  (m': Ghost.erased nat)
+  (data: Ghost.erased (Seq.seq U8.t){Seq.length data == Ghost.reveal m'})
+  (t8: Spec.table_buf)
+  (l: U32.t{(U32.v l) % 4 > 0})
+  (r: U32.t{U32.v r < (U32.v l) % 4})
+  (buf: B.buffer U8.t{B.length buf == U32.v l})
   (crc: U32.t):
-  ST.Stack (U32.t * B.buffer U8.t)
+  ST.Stack ((U32.t & (B.buffer U8.t)) & (Ghost.erased (Seq.seq U8.t)))
   (decreases (U32.v r) - ((U32.v l) % 4))
   (requires fun h ->
-    let curr = crc32_u8_to_bits #m #0 (data @| Seq.slice 0 (B.as_seq h buf) r) crc false in
     B.live h buf /\
     table_correct 8 h t8 /\
-    crc32_matched
-      (crc32_u8_to_bits #m #0 data (Seq.empty #bool))
-      crc false)
+    B.disjoint t8 buf /\
+    (Ghost.reveal m') == (Ghost.reveal m) + (U32.v r) /\
+    Seq.equal data (prev @| (Seq.slice (B.as_seq h buf) 0 (U32.v r))) /\
+    crc32_matched m' data crc false)
   (ensures fun h0 res h1 ->
-    let curr = crc32_u8_to_bits
-      #(m + ((U32.v l) % 4))
-      #0
-      (data @| (Seq.slice (B.as_seq h1 buf) 0 ((U32.v l) % 4)))
-      (Seq.empty #bool) in
-    M.modifies M.loc_none h0 h1 /\
-    crc32_matched #_ curr (fst res) false) =
+    let crc' = fst (fst res) in
+    let buf' = snd (fst res) in
+    let data' = Ghost.reveal (snd res) in
+    B.modifies B.loc_none h0 h1 /\
+    (B.length buf') % 4 == 0 /\
+    Seq.length data' == (m + ((U32.v l) % 4)) /\
+    Seq.equal data' (prev @| (Seq.slice (B.as_seq h1 buf) 0 ((U32.v l) % 4))) /\
+    crc32_matched (m + ((U32.v l) % 4)) data' crc' false) =
   let open U32 in
-  if r <^ (l %^ 4ul) then begin
-    admit();
-    do1_remain t8 l buf m data
-      (r +^ 1ul)
-      (do1
-        t8
-        (crc32_u8_to_bits #m #0 data (Seq.empty #bool))
-        crc
-        (B.index buf r))
+  let (crc', data') = do1 m' data t8 crc (B.index buf r) in
+  if r +^ 1ul <^ l %^ 4ul then begin
+    do1_remain m prev (m + ((v r) + 1)) data' t8 l (r +^ 1ul) buf crc'
   end else begin
-    (crc, buf)
+    let buf' = B.sub buf (r +^ 1ul) (l -^ (r +^ 1ul)) in
+    ((crc', buf'), data')
   end
 
-let crc32_impl #n prev t8 t16 t24 t32 crc buf len =
+inline_for_extraction
+private let dword_seq_to_u32 (a b c d: U8.t): Tot(crc32_data_dword a b c d) =
+  let a' = Cast.uint8_to_uint32 a in
+  let b' = Cast.uint8_to_uint32 b in
+  let c' = Cast.uint8_to_uint32 c in
+  let d' = Cast.uint8_to_uint32 d in
+  cast_zero_prefix (U8.v a) 32;
+  cast_zero_prefix (U8.v b) 32;
+  cast_zero_prefix (U8.v c) 32;
+  cast_zero_prefix (U8.v d) 32;
+  let open U32 in
+  a' ^^ (b' <<^ 8ul) ^^ (c' <<^ 16ul) ^^ (d' <<^ 24ul)
+
+let do4_logxor
+  (#m: nat)
+  (data: Seq.seq U8.t{Seq.length data == m})
+  (crc: U32.t)
+  (a b c d: U8.t): Lemma
+  (requires crc32_matched m data crc false)
+  (ensures
+    (m == 0 ==>
+      UInt.to_vec (U32.v (U32.logxor crc (dword_seq_to_u32 a b c d))) ==
+      (BV.ones_vec #32 +@ (UInt.to_vec (U32.v (dword_seq_to_u32 a b c d))))) /\
+    (m > 0 ==>
+      UInt.to_vec (U32.v (U32.logxor crc (dword_seq_to_u32 a b c d))) ==
+      poly_mod (
+        (zero_vec_r (8 * m) (UInt.to_vec (U32.v (dword_seq_to_u32 a b c d)))) +@
+        (crc32_data_to_bits m data)))) =
+  let open U32 in
+  let sum = dword_seq_to_u32 a b c d in
+  let vsum = UInt.to_vec (v sum) in
+  let prev_len = if m > 0 then 32 + 8 * m else 0 in
+  if m = 0 then
+    ()
+  else
+    calc (==) {
+      UInt.to_vec (U32.v (U32.logxor crc (dword_seq_to_u32 a b c d)));
+      =={}
+      (UInt.to_vec (v crc)) +@ (UInt.to_vec (v sum));
+      =={poly_mod_zero_suffix (UInt.to_vec (v sum)) (prev_len - 32)}
+      poly_mod (crc32_data_to_bits m data) +@ poly_mod (zero_vec_r (prev_len - 32) vsum);
+      =={poly_mod_add (crc32_data_to_bits m data) (zero_vec_r (prev_len - 32) vsum)}
+      poly_mod ((crc32_data_to_bits m data) +@ (zero_vec_r (prev_len - 32) vsum));
+    }
+
+#set-options "--z3rlimit 120 --fuel 0 --ifuel 0"
+private let do4_table_lookup
+  (r: U32.t) (t0: U32.t{
+    let open U32 in poly_mod_correct 32 (r &^ 0xFFul) t0
+  }) (t1: U32.t{
+    let open U32 in poly_mod_correct 24 ((r >>^ 8ul) &^ 0xFFul) t1
+  }) (t2: U32.t{
+    let open U32 in poly_mod_correct 16 ((r >>^ 16ul) &^ 0xFFul) t2
+  }) (t3: U32.t{
+    let open U32 in poly_mod_correct 8 (r >>^ 24ul) t3
+  }) (sum: U32.t{
+    let open U32 in sum == t0 ^^ t1 ^^ t2 ^^ t3
+  }): Lemma
+  (ensures poly_mod (zero_vec_l 32 (UInt.to_vec (U32.v r))) == UInt.to_vec (U32.v sum)) =
+  let open U32 in
+  let r0 = r &^ 0xFFul in
+  let r1 = (r >>^ 8ul) &^ 0xFFul in
+  let r2 = (r >>^ 16ul) &^ 0xFFul in
+  let r3 = r >>^ 24ul in
+  let vr = v r in let vr0 = v r0 in let vr1 = v r1 in let vr2 = v r2 in let vr3 = v r3 in
+  let vr' = UInt.to_vec vr in let vr0' = UInt.to_vec vr0 in let vr1' = UInt.to_vec vr1 in
+  let vr2' = UInt.to_vec vr2 in let vr3' = UInt.to_vec vr3 in
+
+  logand_256 r; logand_256 (r >>^ 8ul); logand_256 (r >>^ 16ul);
+
+  poly_mod_correct_eq 32 r0 t0; poly_mod_correct_eq 24 r1 t1;
+  poly_mod_correct_eq 16 r2 t2; poly_mod_correct_eq 8 r3 t3;
+
+  poly_mod_zero_suffix (zero_vec_l 24 vr1') 8;
+  poly_mod_zero_suffix (zero_vec_l 16 vr2') 16;
+  poly_mod_zero_suffix (zero_vec_l 8 vr3') 24;
+
+  poly_mod_add (zero_vec_l 32 vr0') (zero_vec_r 8 (zero_vec_l 24 vr1'));
+  poly_mod_add
+    ((zero_vec_l 32 vr0') +@ zero_vec_r 8 (zero_vec_l 24 vr1'))
+    (zero_vec_r 16 (zero_vec_l 16 vr2'));
+  poly_mod_add
+    ((zero_vec_l 32 vr0') +@
+     zero_vec_r 8 (zero_vec_l 24 vr1') +@
+     zero_vec_r 16 (zero_vec_l 16 vr2'))
+    (zero_vec_r 24 (zero_vec_l 8 vr3'));
+    
+  assert(Seq.equal (zero_vec_l 32 vr') (
+    (zero_vec_l 32 vr0') +@
+    (zero_vec_r 8 (zero_vec_l 24 vr1')) +@
+    (zero_vec_r 16 (zero_vec_l 16 vr2')) +@
+    (zero_vec_r 24 (zero_vec_l 8 vr3'))
+  ));
+
+  assert(Seq.equal
+    (UInt.to_vec (v sum))
+    ((poly_mod_u32 32 r0) +@
+    (poly_mod_u32 24 r1) +@
+    (poly_mod_u32 16 r2) +@
+    (poly_mod_u32 8 r3)))
+
+#set-options "--z3rlimit 120 --fuel 0 --ifuel 0"
+inline_for_extraction
+private let do4
+  (#m: Ghost.erased nat)
+  (data: Ghost.erased (Seq.seq U8.t){Seq.length data == Ghost.reveal m})
+  (t8 t16 t24 t32: Spec.table_buf)
+  (crc: U32.t)
+  (a b c d: U8.t):
+  ST.Stack (U32.t & (Ghost.erased (Seq.seq U8.t)))
+  (requires fun h ->
+    table_group_correct h t8 t16 t24 t32 /\
+    crc32_matched m data crc false)
+  (ensures fun h0 res h1 ->
+    let crc' = fst res in
+    let data' = Ghost.reveal (snd res) in
+    B.modifies B.loc_none h0 h1 /\
+    data' == data @| (Seq.init 4 (fun i -> match i with | 0 -> a | 1 -> b | 2 -> c | 3 -> d)) /\
+    crc32_matched (m + 4) data' crc' false) =
+  let open U32 in
+  let dw = dword_seq_to_u32 a b c d in
+  let dw' = Ghost.hide (UInt.to_vec (v dw)) in
+  let r = crc ^^ dw in
+  let r' = Ghost.hide (UInt.to_vec (v r)) in
+  let r0 = r &^ 0xFFul in
+  let r1 = (r >>^ 8ul) &^ 0xFFul in
+  let r2 = (r >>^ 16ul) &^ 0xFFul in
+  let r3 = r >>^ 24ul in
+  UInt.logand_le (v r) 255;
+  UInt.logand_le (v (r >>^ 8ul)) 255;
+  UInt.logand_le (v (r >>^ 16ul)) 255;
+  Math.lemma_div_lt (v r) 32 24;
+  do4_logxor #m data crc a b c d;
+
+  let t0 = t32.(r0) in let t1 = t24.(r1) in let t2 = t16.(r2) in let t3 = t8.(r3) in
+  let crc' = t0 ^^ t1 ^^ t2 ^^ t3 in
+  do4_table_lookup r t0 t1 t2 t3 crc';
+
+  let seq_32bit = Ghost.hide (crc32_dword_seq a b c d) in
+  let buf:
+    Ghost.erased (BV.bv_t (if m > 0 then 32 + 8 * m else 0)) =
+    Ghost.hide (crc32_data_to_bits m data) in
+
+  assert(poly_mod (zero_vec_l 32 (UInt.to_vec (U32.v r))) == (UInt.to_vec (U32.v crc')));
+  crc32_data_to_bits_append m 4 data seq_32bit;
+  crc32_data_to_bits_32bit m data buf dw;
+  if Ghost.reveal m > 0 then
+    poly_mod_zero_prefix ((zero_vec_r (8 * m) dw') +@ buf) 32
+  else
+    assert(Seq.equal seq_32bit (data @| seq_32bit));
+
+  (crc', Ghost.hide (data @| seq_32bit))
+
+let crc32_impl m data t8 t16 t24 t32 crc buf len =
   let open U32 in
   ST.push_frame ();
+  let crc' = crc ^^ 0xfffffffful in
+  crc32_matched_xor_inv_1 m data crc;
+  let ((c0, buf'), data') = if len %^ 4ul >^ 0ul then
+    do1_remain m data m data t8 len 0ul buf crc'
+  else
+    ((crc', buf), data)
+  in
   admit();
   ST.pop_frame ();
-  0ul
+  c0
